Add methods to cover CWEs for file handling

src/tests/filestream/fileio_with_sensitive_files.dfy
@@ -3,6 +3,8 @@ newtype{:nativeType "byte"} byte = i:int | 0 <= i < 0x100
 newtype{:nativeType "int"} int32 = i:int | -0x80000000 <= i < 0x80000000
 newtype{:nativeType "int"} nat32 = i:int | 0 <= i < 0x80000000
 newtype{:nativeType "int"} maxPath = i:int | 0 <= i < 256
+datatype path = path(length: int, data: seq<char>)
+
 // newtype{:nativeType "char"} validPathChar = c:char | c
 // newtype{:nativeType "path"} path = c:char | 
 // TODO: Define a new datatype for path (os.path type is a string)
@@ -30,12 +32,19 @@ class FileStream
   function {:axiom} Capabilities():(string, string) reads this
   function{:axiom} Path():string reads this
   constructor{:axiom} () requires false
-
+  function{:axiom} FileIsValid():bool reads this
+  function{:axiom} DirIsValid():bool reads this
+  const sensitivePaths := ["/usr", "/System", "/bin", "/sbin", "/var", "/usr/local"]
+  const nonSensitiveFiles := ["safeFile_1.txt", "safeFile_2.txt", "safeFile_3.txt", "bar.txt", "baz.txt"]
+  const fileMaxLength := 255
+  const dirMaxLength := 4096
+  
   // static method{:axiom} Open(name:array<char>, ghost env:HostEnvironment, access:array<char>)
-    static method{:axiom} Open(name:array<char>, ghost env:HostEnvironment)
+    // static method{:axiom} Open(name:seq<char>, ghost env:HostEnvironment)
+  static method{:axiom} Open(name:array<char>, ghost env:HostEnvironment)
     returns(ok:bool, f:FileStream)
     // CannotAccessSensitiveFiles(l: ["bar.txt", "baz.txt"], access: ["bar.txt", "baz.txt"])
-    requires name[..] in ["bar.txt", "baz.txt"]
+    requires name[..] in ["safeFile_1.txt", "safeFile_2.txt", "safeFile_3.txt", "bar.txt", "baz.txt"]
     // requires access[..] in ["read", "write"]
     // requires capabilities in [("bar.txt", "write")]
     requires env.ok.ok()
@@ -43,8 +52,19 @@ class FileStream
     ensures  env.ok.ok() == ok
     ensures  ok ==> fresh(f) && f.env == env && f.IsOpen() && f.Name() == name[..]
 
+  // predicate isSubstring(p: path)
+  // ensures forall i | i in sensitivePaths :: 0 < i < path.length
+  // ensures exists substring :: substring in sensitivePaths && exists i :: 0 < i < (path.length - i) && forall j :: 0 <= j < |i| ==> 
+  // {
+  //   forall d | d in sensitivePaths :: d 
+  // }
+  // A function that checks if any input path is valid
+  // function{:axiom} validatePath(p:path, ghost env:HostEnvironment): bool
+  //   requires p.data[..] !in sensitivePaths
+  //   requires < |p.data|
+
   method{:axiom} Close() returns(ok:bool)
-    requires Name() in ["bar.txt", "baz.txt"]
+    requires Name() in nonSensitiveFiles
     // requires Access() in ["read", "write"]
     // requires Capabilities in [("bar.txt", ["read, write"]), ("baz.txt", ["read"])]
     requires env.ok.ok()
@@ -58,7 +78,7 @@ class FileStream
     requires env.ok.ok()
     requires IsOpen()
     requires 0 <= start as int <= end as int <= buffer.Length
-    requires Name() in ["bar.txt", "baz.txt"]
+    requires Name() in nonSensitiveFiles
     // requires Access() in ["read", "write"]
     // requires Capabilities() in [("bar.txt", ["read, write"]), ("baz.txt", ["read"])]
     modifies env.ok
@@ -70,10 +90,12 @@ class FileStream
     ensures  ok ==> IsOpen()
 
   method{:axiom} Write(fileOffset:nat32, buffer:array<byte>, start:int32, end:int32) returns(ok:bool)
+  // method{:axiom} Write(fileOffset:nat32, buffer:seq<byte>, start:int32, end:int32) returns(ok:bool)
     requires env.ok.ok()
     requires IsOpen()
     requires 0 <= start as int <= end as int <= buffer.Length
-    requires Name() in ["bar.txt", "baz.txt"]
+    // requires 0 <= start as int <= end as int <= |buffer|
+    requires Name() in nonSensitiveFiles
     // requires Access() in ["read", "write"]
     // requires Capabilities in [("bar.txt", ["read, write"]), ("baz.txt", ["read"])]
     modifies this
@@ -93,9 +115,46 @@ class FileStream
     ensures  Name() == old(Name())
     ensures  ok ==> IsOpen()
 
-  method{:axiom} Join(path:seq<char>, file:seq<char>) returns(ok:bool, result:seq<char>)
+function IsValidCharacter(c: char): bool
+{
+    // Valid characters include letters, digits, underscores, hyphens, and periods
+    (c >= 'a' && c <= 'z') ||
+    (c >= 'A' && c <= 'Z') ||
+    (c >= '0' && c <= '9') ||
+    c == '_' ||
+    c == '-' ||
+    c == '.'
+}
+
+predicate IsValidDirName(dirName: seq<char>)
+{
+    // Check if the directory name is not empty
+    0 < |dirName| <= dirMaxLength && 
+    // Check if each character in the directory name is a valid character
+    forall i :: 0 <= i < |dirName| ==> IsValidCharacter(dirName[i])
+}
+
+predicate IsValidFileName(fileName: seq<char>) 
+{
+    // Check if the filename is not empty 
+    // Check if the filename length is within the specified range
+    3 < |fileName| <= fileMaxLength &&
+    // Check if the filename contains only allowed characters (e.g., letters, digits, underscores, hyphens, periods)
+    forall c :: 0 <= c < |fileName| ==> IsValidCharacter(fileName[c]) &&
+    // Check if the filename does not start or end with a period (.)
+    fileName[0] != '.' && fileName[|fileName| - 1] != '.' &&
+    // Check if the filename is not one of the reserved names
+    !(fileName in {"CON", "PRN", "AUX", "NUL", "COM1", "COM2", "COM3", "COM4", "LPT1", "LPT2", "LPT3", "LPT4", "LPT5", "LPT6", "LPT7", "LPT8", "LPT9"})
+}
+
+method{:axiom} Join(path:seq<char>, file:seq<char>) returns(ok:bool, result:seq<char>)
+  //predicate for IsFileValid
+  //predicate for IsPathValid
+  //predicate for IsPathSensitive --> can swap with different implementations
   requires path[..] in ["/Users/pari/pcc-llms/src/"]
+  requires path !in sensitivePaths
   requires file[..] in ["foo.txt", "foobar.txt"]
+  requires IsValidFileName(file) == true
   requires env.ok.ok()
   requires forall i :: 0 <= i < |path| ==> !(((i < |path| - 1 && ((path[i] == '.' && path[i + 1] == '.') 
   || (path[i] == '/' && path[i + 1] == '/'))) || (i < |path| - 2 && path[i] == '.' && path[i + 1] == '.' && path[i + 2] == '/')))
@@ -111,47 +170,46 @@ class FileStream
   ensures |result| <= |path| + |file|
   ensures  ok ==> IsOpen()
 
-  method IsFilenameValid(filename: seq<char>) returns (ok: bool)
-  requires env.ok.ok()
-  requires IsOpen()
-  requires forall i :: 0 <= i < |filename| ==> ((filename[i] >= 'a' && filename[i] <= 'z') ||
-   (filename[i] >= 'A' && filename[i] <= 'Z') || (filename[i] >= '0' && filename[i] <= '9') ||
-    filename[i] == '_' || filename[i] == '.' || filename[i] == '-')
+  // method{:axiom} IsFilenameValid(filename: seq<char>) returns (ok: bool)
+  // requires env.ok.ok()
+  // requires IsOpen()
+  // requires forall i :: 0 <= i < |filename| ==> ((filename[i] >= 'a' && filename[i] <= 'z') ||
+  //  (filename[i] >= 'A' && filename[i] <= 'Z') || (filename[i] >= '0' && filename[i] <= '9') ||
+  //   filename[i] == '_' || filename[i] == '.' || filename[i] == '-')
+  // modifies this
+  // modifies env.ok
+  // ensures  env == old(env)
+  // ensures  env.ok.ok() == ok
+  // ensures  Name() == old(Name())
+  // ensures  ok ==> IsOpen()
+
+  // method{:axiom} GetCWD(dirname: seq<char>) returns (ok: bool)
+  // requires env.ok.ok()
+  // requires IsOpen()
+  // ensures dirname == old(dirname)
+  // ensures  env == old(env)
+  // ensures  env.ok.ok() == ok
+  // ensures  Name() == old(Name())
+  // ensures  ok ==> IsOpen()
+
+  method{:axiom} GetCWD(currDir: seq<char>, isCurrDir: seq<char>) returns (isEqual: bool)
   modifies this
   modifies env.ok
-  ensures  env == old(env)
-  ensures  env.ok.ok() == ok
-  ensures  Name() == old(Name())
-  ensures  ok ==> IsOpen()
-
-  method IsDirNameValid(dirname: seq<char>) returns (ok:bool)
   requires env.ok.ok()
-  requires |dirname| > 0 && |dirname| < 256
-  modifies this
-  modifies env.ok
-  ensures  env == old(env)
-  ensures  env.ok.ok() == ok
-
-  method GetCWD(dirname: seq<char>) returns (ok: bool)
-  requires env.ok.ok()
-  requires IsOpen()
-  ensures dirname == old(dirname)
-  ensures  env == old(env)
-  ensures  env.ok.ok() == ok
-  ensures  Name() == old(Name())
-  ensures  ok ==> IsOpen()
-
-  method checkCWD(oldDirName: seq<char>, newDirName: seq<char>) returns (isEqual: bool)
-  requires env.ok.ok()
-  requires IsOpen()
-  ensures oldDirName == old(oldDirName)
-  requires oldDirName == newDirName
-  requires oldDirName in ["/Users/pari/pcc-llms/src/examples/generated_codes"]
+  requires currDir !in sensitivePaths
+  requires currDir == isCurrDir
+  requires currDir in ["/Users/pari/pcc-llms/src/examples/generated_codes"]
   ensures  env == old(env)
   ensures  env.ok.ok() == isEqual
   ensures  Name() == old(Name())
-  ensures  isEqual ==> IsOpen()
+  ensures  isEqual ==> currDir == isCurrDir
 
+method{:axiom} rmdir (dirname: seq<char>)
+  modifies this
+  modifies env.ok
+  requires env.ok.ok()
+  requires dirname !in sensitivePaths
+// TODO: How to link axioms to python functions
 // TODO: Basically Join is similar to concatenation of two string
   // method concatenation(str1: seq<char>, str2: seq<char>) returns (ok: bool, result: seq<char>) 
   // requires env.ok.ok()
